current

code/experimental/poly1305/Hacl.Impl.Poly1305.Field128.fst
@@ -6,31 +6,33 @@ open FStar.HyperStack.All
 open Lib.IntTypes
 open Lib.Buffer
 open Lib.ByteBuffer
-open Lib.Vec128
+open Lib.IntVector
 
-let felem = lbuffer vec128 5ul
-let felem_wide = lbuffer vec128 5ul
-let precomp_r = lbuffer vec128 20ul
+let uint64x2 = vec_t U64 2
+let zero = vec_zero U64 2
+let felem = lbuffer uint64x2 5ul
+let felem_wide = lbuffer uint64x2 5ul
+let precomp_r = lbuffer uint64x2 20ul
 
 
 inline_for_extraction
-let mask26 = vec128_load64 (u64 0x3ffffff)
+let mask26 = vec_load (u64 0x3ffffff) 2
 inline_for_extraction
-let mask14 = vec128_load64 (u64 0x3fff)
+let mask14 = vec_load (u64 0x3fff) 2
 
 inline_for_extraction
 val create_felem: unit -> StackInline felem
 		       (requires (fun h -> True))
-		       (ensures (fun h0 b h1 -> live h1 b /\ stack_allocated b h0 h1 (Lib.Sequence.create 5 vec128_zero)))
+		       (ensures (fun h0 b h1 -> live h1 b /\ stack_allocated b h0 h1 (Lib.Sequence.create 5 zero)))
 inline_for_extraction
-let create_felem () = create (size 5) vec128_zero 
+let create_felem () = create (size 5) zero
 
 inline_for_extraction
 val create_wide: unit -> StackInline felem_wide
 		       (requires (fun h -> True))
-		       (ensures (fun h0 b h1 -> live h1 b /\ stack_allocated b h0 h1 (Lib.Sequence.create 5 vec128_zero)))
+		       (ensures (fun h0 b h1 -> live h1 b /\ stack_allocated b h0 h1 (Lib.Sequence.create 5 zero)))
 inline_for_extraction
-let create_wide () = create (size 5) vec128_zero 
+let create_wide () = create (size 5) zero
 
 
 inline_for_extraction
@@ -39,8 +41,9 @@ val set_bit: f:felem -> i:size_t{size_v i < 130} -> Stack unit
 		   (ensures (fun h0 _ h1 -> modifies (loc f) h0 h1))
 let set_bit f i = 
   let b = u64 1 <<. (i %. size 26) in
-  let mask = vec128_load64 b in
-  f.(i /. size 26) <- vec128_or f.(i /. size 26) mask
+  let mask = vec_load b 2 in
+  let fi = f.(i /. size 26) in
+  f.(i /. size 26) <- vec_or fi mask
 
 inline_for_extraction
 val set_bit128: f:felem -> Stack unit
@@ -48,19 +51,20 @@ val set_bit128: f:felem -> Stack unit
 		   (ensures (fun h0 _ h1 -> modifies (loc f) h0 h1))
 let set_bit128 f = 
   let b = u64 0x1000000 in
-  let mask = vec128_load64  b in
-  f.(size 4) <- vec128_or f.(size 4) mask
+  let mask = vec_load  b 2 in
+  let f4 = f.(4ul) in
+  f.(size 4) <- vec_or f4 mask
 
 inline_for_extraction
 val set_zero: f:felem -> Stack unit
                    (requires (fun h -> live h f))
 		   (ensures (fun h0 _ h1 -> modifies (loc f) h0 h1))
 let set_zero f = 
-    f.(size 0) <- vec128_zero;
-    f.(size 1) <- vec128_zero;
-    f.(size 2) <- vec128_zero;
-    f.(size 3) <- vec128_zero;
-    f.(size 4) <- vec128_zero
+    f.(size 0) <- zero;
+    f.(size 1) <- zero;
+    f.(size 2) <- zero;
+    f.(size 3) <- zero;
+    f.(size 4) <- zero
 
 inline_for_extraction
 val copy_felem: f1:felem -> f2:felem -> Stack unit
@@ -74,17 +78,17 @@ let copy_felem f1 f2 =
     f1.(size 4) <- f2.(size 4)
 
 inline_for_extraction
-val load_felem: f:felem -> lo:vec128 -> hi:vec128 -> Stack unit
+val load_felem: f:felem -> lo:uint64x2 -> hi:uint64x2 -> Stack unit
                    (requires (fun h -> live h f))
 		   (ensures (fun h0 _ h1 -> modifies (loc f) h0 h1))
 let load_felem f b1 b2 =
-    let lo = vec128_interleave_low64 b1 b2 in
-    let hi = vec128_interleave_high64 b1 b2 in
-    f.(size 0) <- vec128_and lo mask26;
-    f.(size 1) <- vec128_and (vec128_shift_right64 lo (size 26)) mask26;
-    f.(size 2) <- vec128_or (vec128_shift_right64 lo (size 52)) (vec128_shift_left64 (vec128_and hi mask14) (size 12));
-    f.(size 3) <- vec128_and (vec128_shift_right64 hi (size 14)) mask26;
-    f.(size 4) <- vec128_shift_right64 hi (size 40)
+    let lo = vec_interleave_low b1 b2 in
+    let hi = vec_interleave_high b1 b2 in
+    f.(size 0) <- vec_and lo mask26;
+    f.(size 1) <- vec_and (vec_shift_right lo (size 26)) mask26;
+    f.(size 2) <- vec_or (vec_shift_right lo (size 52)) (vec_shift_left (vec_and hi mask14) (size 12));
+    f.(size 3) <- vec_and (vec_shift_right hi (size 14)) mask26;
+    f.(size 4) <- vec_shift_right hi (size 40)
 
 
 #reset-options "--z3rlimit 50"
@@ -106,15 +110,15 @@ let fadd out f1 f2 =
   let f22 = f2.(size 2) in
   let f23 = f2.(size 3) in
   let f24 = f2.(size 4) in
-  out.(size 0) <- vec128_add64 f10 f20;
-  out.(size 1) <- vec128_add64 f11 f21;
-  out.(size 2) <- vec128_add64 f12 f22;
-  out.(size 3) <- vec128_add64 f13 f23;
-  out.(size 4) <- vec128_add64 f14 f24
+  out.(size 0) <- vec_add_mod f10 f20;
+  out.(size 1) <- vec_add_mod f11 f21;
+  out.(size 2) <- vec_add_mod f12 f22;
+  out.(size 3) <- vec_add_mod f13 f23;
+  out.(size 4) <- vec_add_mod f14 f24
 
 //[@ CInline]
 inline_for_extraction
-val smul_felem: out:felem_wide -> u1:vec128 -> f2:felem -> Stack unit
+val smul_felem: out:felem_wide -> u1:uint64x2 -> f2:felem -> Stack unit
                    (requires (fun h -> live h out /\ live h f2))
 		   (ensures (fun h0 _ h1 -> modifies (loc out) h0 h1))
 [@ CInline]
@@ -124,16 +128,16 @@ let smul_felem out u1 f2 =
   let f22 = f2.(size 2) in
   let f23 = f2.(size 3) in
   let f24 = f2.(size 4) in
-  out.(size 0) <- vec128_mul64 f20 u1;
-  out.(size 1) <- vec128_mul64 f21 u1;
-  out.(size 2) <- vec128_mul64 f22 u1;
-  out.(size 3) <- vec128_mul64 f23 u1;
-  out.(size 4) <- vec128_mul64 f24 u1
+  out.(size 0) <- vec_mul_mod f20 u1;
+  out.(size 1) <- vec_mul_mod f21 u1;
+  out.(size 2) <- vec_mul_mod f22 u1;
+  out.(size 3) <- vec_mul_mod f23 u1;
+  out.(size 4) <- vec_mul_mod f24 u1
 
 
 //[@ CInline]
 inline_for_extraction
-val smul_add_felem: out:felem_wide -> u1:vec128 -> f2:felem -> Stack unit
+val smul_add_felem: out:felem_wide -> u1:uint64x2 -> f2:felem -> Stack unit
                    (requires (fun h -> live h out /\ live h f2))
 		   (ensures (fun h0 _ h1 -> modifies (loc out) h0 h1))
 [@ CInline]
@@ -148,11 +152,11 @@ let smul_add_felem out u1 f2 =
   let o2 = out.(size 2) in
   let o3 = out.(size 3) in
   let o4 = out.(size 4) in
-  out.(size 0) <- vec128_add64 o0 (vec128_mul64 f20 u1);
-  out.(size 1) <- vec128_add64 o1 (vec128_mul64 f21 u1);
-  out.(size 2) <- vec128_add64 o2 (vec128_mul64 f22 u1);
-  out.(size 3) <- vec128_add64 o3 (vec128_mul64 f23 u1);
-  out.(size 4) <- vec128_add64 o4 (vec128_mul64 f24 u1)
+  out.(size 0) <- vec_add_mod o0 (vec_mul_mod f20 u1);
+  out.(size 1) <- vec_add_mod o1 (vec_mul_mod f21 u1);
+  out.(size 2) <- vec_add_mod o2 (vec_mul_mod f22 u1);
+  out.(size 3) <- vec_add_mod o3 (vec_mul_mod f23 u1);
+  out.(size 4) <- vec_add_mod o4 (vec_mul_mod f24 u1)
 
 inline_for_extraction
 val mul_felem: out:felem_wide -> f1:felem -> r:felem -> r5:felem  -> Stack unit
@@ -192,13 +196,13 @@ let mul_felem out f1 r r5 =
 
 
 inline_for_extraction
-val carry26: l:vec128 -> cin:vec128 ->  (r:vec128 * cout:vec128)
+val carry26: l:uint64x2 -> cin:uint64x2 ->  (r:uint64x2 * cout:uint64x2)
 let carry26 l cin = 
-    let l = vec128_add64 l cin in
-    (vec128_and l mask26, vec128_shift_right64 l (size 26))
+    let l = vec_add_mod l cin in
+    (vec_and l mask26, vec_shift_right l (size 26))
 
 inline_for_extraction
-val carry26_wide: l:vec128 -> cin:vec128 ->  (r:vec128 * cout:vec128)
+val carry26_wide: l:uint64x2 -> cin:uint64x2 ->  (r:uint64x2 * cout:uint64x2)
 let carry26_wide l cin = carry26 l cin
 
 //[@ CInline]
@@ -213,13 +217,13 @@ let carry_wide_felem out inp =
   let i2 = inp.(size 2) in
   let i3 = inp.(size 3) in
   let i4 = inp.(size 4) in
-  let tmp0,carry = carry26_wide i0 vec128_zero in
+  let tmp0,carry = carry26_wide i0 zero in
   let tmp1,carry = carry26_wide i1 carry in
   let tmp2,carry = carry26_wide i2 carry in
   let tmp3,carry = carry26_wide i3 carry in
   let tmp4,carry = carry26_wide i4 carry in
-  let tmp0,carry = carry26 tmp0 (vec128_smul64 carry (u64 5)) in
-  let tmp1 = vec128_add64 tmp1 carry in
+  let tmp0,carry = carry26 tmp0 (vec_smul_mod carry (u64 5)) in
+  let tmp1 = vec_add_mod tmp1 carry in
   out.(size 0) <- tmp0;
   out.(size 1) <- tmp1;
   out.(size 2) <- tmp2;
@@ -238,11 +242,11 @@ let carry_felem f =
   let f2 = f.(size 2) in
   let f3 = f.(size 3) in
   let f4 = f.(size 4) in
-  let tmp0,carry = carry26 f0 vec128_zero in
+  let tmp0,carry = carry26 f0 zero in
   let tmp1,carry = carry26 f1 carry in
   let tmp2,carry = carry26 f2 carry in
   let tmp3,carry = carry26 f3 carry in
-  let tmp4 = vec128_add64 f4 carry in
+  let tmp4 = vec_add_mod f4 carry in
   f.(size 0) <- tmp0;
   f.(size 1) <- tmp1;
   f.(size 2) <- tmp2;
@@ -261,9 +265,9 @@ let carry_top_felem f =
   let f2 = f.(size 2) in
   let f3 = f.(size 3) in
   let f4 = f.(size 4) in
-  let tmp4,carry = carry26 f4 vec128_zero in
-  let tmp0,carry = carry26 f0 (vec128_smul64 carry (u64 5)) in
-  let tmp1 = vec128_add64 f1 carry in
+  let tmp4,carry = carry26 f4 zero in
+  let tmp0,carry = carry26 f0 (vec_smul_mod carry (u64 5)) in
+  let tmp1 = vec_add_mod f1 carry in
   f.(size 0) <- tmp0;
   f.(size 1) <- tmp1;
   f.(size 4) <- tmp4  
@@ -317,11 +321,16 @@ val precompute_shift_reduce: f1:felem -> f2:felem -> Stack unit
                    (requires (fun h -> live h f1 /\ live h f2))
 		   (ensures (fun h0 _ h1 -> modifies (loc f1) h0 h1))
 let precompute_shift_reduce f1 f2 = 
-    f1.(size 0) <- vec128_smul64 f2.(size 0) (u64 5);
-    f1.(size 1) <- vec128_smul64 f2.(size 1) (u64 5);
-    f1.(size 2) <- vec128_smul64 f2.(size 2) (u64 5);
-    f1.(size 3) <- vec128_smul64 f2.(size 3) (u64 5);
-    f1.(size 4) <- vec128_smul64 f2.(size 4) (u64 5)
+    let f20 = f2.(size 0) in
+    let f21 = f2.(size 1) in
+    let f22 = f2.(size 2) in
+    let f23 = f2.(size 3) in
+    let f24 = f2.(size 4) in
+    f1.(size 0) <- vec_smul_mod f20 (u64 5);
+    f1.(size 1) <- vec_smul_mod f21 (u64 5);
+    f1.(size 2) <- vec_smul_mod f22 (u64 5);
+    f1.(size 3) <- vec_smul_mod f23 (u64 5);
+    f1.(size 4) <- vec_smul_mod f24 (u64 5)
 
 inline_for_extraction
 val fmul_rn_normalize: out:felem -> p:precomp_r -> Stack unit
@@ -335,19 +344,24 @@ let fmul_rn_normalize out p =
     let r = sub p (size 0) (size 5) in
     let r2 = sub p (size 10) (size 5) in
     let r2_5 = sub p (size 15) (size 5) in
-    r2.(size 0) <- Lib.Vec128.vec128_interleave_low64 r2.(size 0) r.(size 0);
-    r2.(size 1) <- Lib.Vec128.vec128_interleave_low64 r2.(size 1) r.(size 1);
-    r2.(size 2) <- Lib.Vec128.vec128_interleave_low64 r2.(size 2) r.(size 2);
-    r2.(size 3) <- Lib.Vec128.vec128_interleave_low64 r2.(size 3) r.(size 3);
-    r2.(size 4) <- Lib.Vec128.vec128_interleave_low64 r2.(size 4) r.(size 4);
+    r2.(size 0) <- vec_interleave_low r2.(size 0) r.(size 0);
+    r2.(size 1) <- vec_interleave_low r2.(size 1) r.(size 1);
+    r2.(size 2) <- vec_interleave_low r2.(size 2) r.(size 2);
+    r2.(size 3) <- vec_interleave_low r2.(size 3) r.(size 3);
+    r2.(size 4) <- vec_interleave_low r2.(size 4) r.(size 4);
     precompute_shift_reduce r2_5 r2;
     mul_felem tmp out r2 r2_5;
     carry_wide_felem out tmp;
-    out.(size 0) <- Lib.Vec128.vec128_add64 out.(size 0) (Lib.Vec128.vec128_shift_right out.(size 0) (size 64));
-    out.(size 1) <- Lib.Vec128.vec128_add64 out.(size 1) (Lib.Vec128.vec128_shift_right out.(size 1) (size 64));
-    out.(size 2) <- Lib.Vec128.vec128_add64 out.(size 2) (Lib.Vec128.vec128_shift_right out.(size 2) (size 64));
-    out.(size 3) <- Lib.Vec128.vec128_add64 out.(size 3) (Lib.Vec128.vec128_shift_right out.(size 3) (size 64));
-    out.(size 4) <- Lib.Vec128.vec128_add64 out.(size 4) (Lib.Vec128.vec128_shift_right out.(size 4) (size 64));
+    let o0 = out.(0ul) in
+    let o1 = out.(1ul) in
+    let o2 = out.(2ul) in
+    let o3 = out.(3ul) in
+    let o4 = out.(4ul) in
+    out.(size 0) <- vec_add_mod o0 (vec_interleave_high o0 o0);
+    out.(size 1) <- vec_add_mod o1 (vec_interleave_high o1 o1);
+    out.(size 2) <- vec_add_mod o2 (vec_interleave_high o2 o2);
+    out.(size 3) <- vec_add_mod o3 (vec_interleave_high o3 o3);
+    out.(size 4) <- vec_add_mod o4 (vec_interleave_high o4 o4);
     carry_felem out;	 
     carry_top_felem out;	 
     pop_frame()
@@ -363,7 +377,7 @@ let load_precompute_r p r0 r1 =
     let r5 = sub p (size 5) (size 5) in
     let r2 = sub p (size 10) (size 5) in
     let r2_5 = sub p (size 15) (size 5) in
-    let r_vec = vec128_load64s r1 r0 in
+    let r_vec = vec_load2 r1 r0 in
     load_felem r r_vec r_vec;
     precompute_shift_reduce r5 r;
     let tmp = create_felem () in
@@ -371,33 +385,6 @@ let load_precompute_r p r0 r1 =
     carry_wide_felem r2 tmp;
     precompute_shift_reduce r2_5 r2;
     pop_frame()
-
-inline_for_extraction
-let vec128_eq_mask (a:vec128) (b:vec128) : vec128
-  = vec128_eq64 a b
-(*  
-  let x = vec128_xor a b in
-    let one = vec128_load64 (u64 1) in
-    let minus_x = vec128_add64 (vec128_lognot x) one in
-    let x_or_minus_x = vec128_or x minus_x in
-    let xnx = vec128_shift_right64 x_or_minus_x (size 63) in
-    let c = vec128_sub64 xnx one in
-    c
-*)
-
-inline_for_extraction
-let vec128_gte_mask (a:vec128) (b:vec128) : vec128
-  = let x = a in
-    let y = b in
-    let one = vec128_load64 (u64 1) in
-    let x_xor_y = vec128_xor x y in
-    let x_sub_y = vec128_sub64 x y in
-    let x_sub_y_xor_y = vec128_xor x_sub_y y in
-    let q = vec128_or x_xor_y x_sub_y_xor_y in
-    let x_xor_q = vec128_xor x q in
-    let x_xor_q_ = vec128_shift_right64 x_xor_q (size 63) in
-    let c = vec128_sub64 x_xor_q_ one in
-    c
 
 inline_for_extraction
 val subtract_p: f:felem -> Stack unit
@@ -409,20 +396,20 @@ let subtract_p f =
   let f2 = f.(size 2) in
   let f3 = f.(size 3) in
   let f4 = f.(size 4) in
-  let mh = vec128_load64 (u64 0x3ffffff) in
-  let ml = vec128_load64 (u64 0x3fffffb) in
-  let mask = vec128_eq_mask f4 mh in
-  let mask = vec128_and mask (vec128_eq_mask f3 mh) in
-  let mask = vec128_and mask (vec128_eq_mask f2 mh) in
-  let mask = vec128_and mask (vec128_eq_mask f1 mh) in
-  let mask = vec128_and mask (vec128_gte_mask f0 ml) in
-  let ph = vec128_and mask mh in
-  let pl = vec128_and mask ml in 
-  f.(size 0) <- vec128_sub64 f0 pl;
-  f.(size 1) <- vec128_sub64 f1 ph;
-  f.(size 2) <- vec128_sub64 f2 ph;
-  f.(size 3) <- vec128_sub64 f3 ph;
-  f.(size 4) <- vec128_sub64 f4 ph
+  let mh = vec_load (u64 0x3ffffff) 2 in
+  let ml = vec_load (u64 0x3fffffb) 2 in
+  let mask = vec_eq_mask f4 mh in
+  let mask = vec_and mask (vec_eq_mask f3 mh) in
+  let mask = vec_and mask (vec_eq_mask f2 mh) in
+  let mask = vec_and mask (vec_eq_mask f1 mh) in
+  let mask = vec_and mask (vec_gte_mask f0 ml) in
+  let ph = vec_and mask mh in
+  let pl = vec_and mask ml in 
+  f.(size 0) <- vec_sub_mod f0 pl;
+  f.(size 1) <- vec_sub_mod f1 ph;
+  f.(size 2) <- vec_sub_mod f2 ph;
+  f.(size 3) <- vec_sub_mod f3 ph;
+  f.(size 4) <- vec_sub_mod f4 ph
 
 inline_for_extraction
 val reduce_felem: f:felem -> Stack unit
@@ -438,8 +425,8 @@ val load_felems_le: f:felem -> b:lbuffer uint8 32ul -> Stack unit
                    (requires (fun h -> live h f /\ live h b))
 		   (ensures (fun h0 _ h1 -> modifies (loc f) h0 h1))
 let load_felems_le f b =
-    let b1 = vec128_load_le (sub b (size 0) (size 16)) in
-    let b2 = vec128_load_le (sub b (size 16) (size 16)) in
+    let b1 = vec_load_le U64 2 (sub b (size 0) (size 16)) in
+    let b2 = vec_load_le U64 2 (sub b (size 16) (size 16)) in
     load_felem f b1 b2
 
 inline_for_extraction
@@ -447,7 +434,7 @@ val load_felem_le: f:felem -> b:lbuffer uint8 16ul -> Stack unit
                    (requires (fun h -> live h f /\ live h b))
 		   (ensures (fun h0 _ h1 -> modifies (loc f) h0 h1))
 let load_felem_le f b = 
-    let b = vec128_load_le b in
+    let b = vec_load_le U64 2 b in
     load_felem f b b
 
 
@@ -457,12 +444,17 @@ val store_felems_le: b:lbuffer uint8 32ul -> f:felem -> Stack unit
 		   (ensures (fun h0 _ h1 -> modifies (loc b |+| loc f) h0 h1))
 let store_felems_le b f = 
     carry_felem f;
-    let f0 = vec128_or (vec128_or f.(size 0) (vec128_shift_left64 f.(size 1) (size 26))) (vec128_shift_left64 f.(size 2) (size 52)) in
-    let f1 = vec128_or (vec128_or (vec128_shift_right64 f.(size 2) (size 12)) (vec128_shift_left64 f.(size 3) (size 14))) (vec128_shift_left64 f.(size 4) (size 40)) in
-    let r0 = vec128_interleave_low64 f0 f1 in
-    let r1 = vec128_interleave_high64 f0 f1 in
-    vec128_store_le (sub b (size 0) (size 16)) r0;
-    vec128_store_le (sub b (size 16) (size 16)) r1
+    let f0 = f.(0ul) in
+    let f1 = f.(1ul) in
+    let f2 = f.(2ul) in
+    let f3 = f.(3ul) in
+    let f4 = f.(4ul) in
+    let f0 = vec_or (vec_or f0 (vec_shift_left f1 (size 26))) (vec_shift_left f2 (size 52)) in
+    let f1 = vec_or (vec_or (vec_shift_right f2 (size 12)) (vec_shift_left f3 (size 14))) (vec_shift_left f4 (size 40)) in
+    let r0 = vec_interleave_low f0 f1 in
+    let r1 = vec_interleave_high f0 f1 in
+    vec_store_le (sub b (size 0) (size 16)) r0;
+    vec_store_le (sub b (size 16) (size 16)) r1
 
 inline_for_extraction
 val store_felem_le: b:lbuffer uint8 16ul -> f:felem -> Stack unit
@@ -470,8 +462,13 @@ val store_felem_le: b:lbuffer uint8 16ul -> f:felem -> Stack unit
 		   (ensures (fun h0 _ h1 -> modifies (loc b |+| loc f) h0 h1))
 let store_felem_le b f = 
     carry_felem f;
-    let f0 = vec128_or (vec128_or f.(size 0) (vec128_shift_left64 f.(size 1) (size 26))) (vec128_shift_left64 f.(size 2) (size 52)) in
-    let f1 = vec128_or (vec128_or (vec128_shift_right64 f.(size 2) (size 12)) (vec128_shift_left64 f.(size 3) (size 14))) (vec128_shift_left64 f.(size 4) (size 40)) in
-    let r0 = vec128_interleave_low64 f0 f1 in
-    vec128_store_le b r0
+    let f0 = f.(0ul) in
+    let f1 = f.(1ul) in
+    let f2 = f.(2ul) in
+    let f3 = f.(3ul) in
+    let f4 = f.(4ul) in
+    let f0 = vec_or (vec_or f0 (vec_shift_left f1 (size 26))) (vec_shift_left f2 (size 52)) in
+    let f1 = vec_or (vec_or (vec_shift_right f2 (size 12)) (vec_shift_left f3 (size 14))) (vec_shift_left f4 (size 40)) in
+    let r0 = vec_interleave_low f0 f1 in
+    vec_store_le b r0
     
